More attempts – no luck

TraceSets.v
@@ -20,6 +20,7 @@ From Coq Require Import Program.Equality.   (* for `dependent induction` *)
 (* which apparently (CTrees) smuggles in UIP(-equivalent) *)
 From Coq Require Import Logic.FunctionalExtensionality. (* for equality of substitutions *)
 From Coq Require Import Relations.
+From Coq Require Import Sets.Ensembles.
 (* From Coq Require Import Classes.RelationClasses. *)
 
 From SymEx Require Import Expr.
@@ -36,6 +37,9 @@ Open Scope com_scope.
 Open Scope string_scope.
 Open Scope trace_scope.
 
+Example X : Var := "x".
+Example Y : Var := "y".
+
 Ltac splits := repeat (try split).
 
 (** Symbolic semantics *)
@@ -47,72 +51,65 @@ Inductive STrace_step : Type :=
 
 Definition STrace : Type := trace STrace_step.
 
-Inductive has_trace__S : Stmt -> STrace -> Prop :=
-| htr_asgn : forall x e,
-    has_trace__S <{x := e}> [STAsgn x e]
-| htr_seq : forall s1 s2 t1 t2,
-    has_trace__S s1 t1 ->
-    has_trace__S s2 t2 ->
-    has_trace__S <{s1 ; s2}> (t1 ++ t2)
-| htr_par_step_left : forall s1 s2 s t1 t,
-    has_trace__S s1 t1 ->
-    has_trace__S <{s2 || s}> t ->
-    has_trace__S <{(s1 ; s2) || s}> (t1 ++ t)
-| htr_par_step_right : forall s1 s2 s t1 t,
-    has_trace__S s1 t1 ->
-    has_trace__S <{s || s2}> t ->
-    has_trace__S <{s || s1 ; s2}> (t1 ++ t)
-| htr_par_left : forall s1 s2 t1 t2,
-    has_trace__S s1 t1 ->
-    has_trace__S s2 t2 ->
-    has_trace__S <{s1 || s2}> (t1 ++ t2)
-| htr_par_right : forall s1 s2 t1 t2,
-    has_trace__S s1 t1 ->
-    has_trace__S s2 t2 ->
-    has_trace__S <{s1 || s2}> (t2 ++ t1)
-| htr_if_true : forall b s1 s2 t1,
-    has_trace__S s1 t1 ->
-    has_trace__S <{if b {s1}{s2}}> ([STCond b] ++ t1)
-| htr_if_false : forall b s1 s2 t2,
-    has_trace__S s2 t2 ->
-    has_trace__S <{if b {s1}{s2}}> ([STCond (BNot b)] ++ t2)
-.
-(* no need for skip, maybe remove it from def if we need to recurse on s*)
+Definition Concatenate (A B: Ensemble STrace) : Ensemble STrace :=
+  fun t => exists t1 t2, t = t1 ++ t2 /\ A t1 /\ B t2.
 
-(** Attempted functional def, runs into non-termination problems in parallel case
- probably redeemable, but not easily *)
-(* Fixpoint trace__S (s:Stmt) (t: STrace) : Prop := *)
-(*   match s with *)
-(*   | <{ x := e }> => t = [STAsgn x e] *)
-(*   | <{ s1 ; s2 }> => *)
-(*       exists t1 t2, t1 ++ t2 = t /\ trace__S s1 t1 /\ trace__S s2 t2 *)
-(*   | <{(s1 ; s2) || s}> => *)
-(*       exists t1 t2, t1 ++ t2 = t /\ trace__S s1 t1 /\ trace__S <{s2 || s}> t2 *)
-(*   | <{s || (s1 ; s2)}> => *)
-(*       exists t1 t2, t1 ++ t2 = t /\ trace__S s1 t1 /\ trace__S <{s || s2}> t2 *)
-(*   | <{ s1 || s2 }> => exists t1 t2 x s s', t = (t1 ++ t2 :: x) /\ trace__S <{s ; s'}> t1 /\ s1 = <{s ; s'}> *)
-(*   | <{if b {s1}{s2}}> => (exists t1, [STCond b] ++ t1 = t /\ trace__S s1 t1) *)
-(*                       \/ (exists t2, [STCond (BNot b)] ++ t2 = t /\ trace__S s2 t2) *)
-(*   | <{skip}> => t = [] *)
-(*   end. *)
-
-
-Example X : Var := "x".
-Example Y : Var := "y".
-Example branch_ex : has_trace__S <{if X <= 1 {Y := X} {Y := 1}}> [STCond <{X <= 1}> ; STAsgn Y X].
+Example concat_ex : In _  (Concatenate
+                                (Singleton _ [STAsgn X 0])
+                                (Union _
+                                      (Singleton _ [STAsgn Y 0])
+                                      (Singleton _ [STAsgn X 1])))
+                         [STAsgn X 0; STAsgn Y 0].
 Proof.
-  assert ([STCond <{X <= 1}> ; STAsgn Y X] = [STCond <{X <= 1}>] ++ [STAsgn Y X]) by reflexivity.
-  rewrite H. apply htr_if_true. apply htr_asgn.
+  exists [STAsgn X 0]. exists [STAsgn Y 0]. splits.
+  apply Union_introl. apply In_singleton.
 Qed.
 
-Example par_x : has_trace__S <{(X := 1 ; Y := 2) || (X := Y ; Y := X)}> [STAsgn X 1 ; STAsgn X Y ; STAsgn Y X ; STAsgn Y 2].
+Example concat_ex' : In _  (Concatenate
+                                (Singleton _ [STAsgn X 0])
+                                (Union _
+                                      (Singleton _ [STAsgn Y 0])
+                                      (Singleton _ [STAsgn X 1])))
+                         [STAsgn X 0; STAsgn X 1].
 Proof.
-  assert ([STAsgn X 1 ; STAsgn X Y ; STAsgn Y X ; STAsgn Y 2] = [STAsgn X 1] ++ [STAsgn X Y ; STAsgn Y X ; STAsgn Y 2]) by reflexivity.
-  rewrite H. apply htr_par_step_left. apply htr_asgn.
-  assert ([STAsgn X Y;STAsgn Y X;STAsgn Y 2] = [STAsgn X Y] ++ [STAsgn Y X;STAsgn Y 2]) by reflexivity.
-  rewrite H0. apply htr_par_step_right. apply htr_asgn.
-  assert ([STAsgn Y X;STAsgn Y 2] = [STAsgn Y X] ++ [STAsgn Y 2]) by reflexivity.
-  rewrite H1. apply htr_par_right; apply htr_asgn.
+  exists [STAsgn X 0]. exists [STAsgn X 1]. splits.
+  apply Union_intror. apply In_singleton.
+Qed.
+
+Inductive is_interleaving : STrace -> STrace -> STrace -> Prop :=
+| both_empty : is_interleaving [] [] []
+| left_empty : forall t, is_interleaving [] t t
+| right_empty : forall t, is_interleaving t [] t
+| left_step : forall t1 t2 t x,
+    is_interleaving t1 t2 t ->
+    is_interleaving (t1::x) t2 (t::x)
+| right_step : forall t1 t2 t x,
+    is_interleaving t1 t2 t ->
+    is_interleaving t1 (t2::x) (t::x)
+.
+
+Definition Interleave (A B: Ensemble STrace) : Ensemble STrace :=
+  fun t => exists t1 t2, is_interleaving t1 t2 t /\ A t1 /\ B t2.
+
+Fixpoint has_trace__S (s:Stmt) : Ensemble STrace :=
+  match s with
+  | <{ x := e }> => Singleton _ [STAsgn x e]
+  | <{ s1 ; s2 }> => Concatenate (has_trace__S s1) (has_trace__S s2)
+  | <{s1 || s2}> => Interleave (has_trace__S s1) (has_trace__S s2)
+  | <{if b {s1}{s2}}> => Union _
+                              (Concatenate (Singleton _ [STCond b]) (has_trace__S s1))
+                              (Concatenate (Singleton _ [STCond (BNot b)]) (has_trace__S s2))
+  | <{ skip }> => Empty_set STrace
+  end.
+
+Example branch_ex : In _ (has_trace__S <{if X <= 1 {Y := X} {Y := 1}}>) [STCond <{X <= 1}> ; STAsgn Y X].
+Proof. unfold has_trace__S, In. simpl. apply Union_introl. eexists. eexists. splits. reflexivity. Qed.
+
+Example par_x : has_trace__S <{(X := 1 ; Y := 2) || (X := Y ; Y := X)}> [STAsgn X 1 ; STAsgn X Y ; STAsgn Y X ; STAsgn Y 2].
+Proof. unfold has_trace__S, In. exists [STAsgn X 1; STAsgn Y 2]. exists [STAsgn X Y; STAsgn Y X]. splits.
+       - repeat constructor.
+       - eexists. eexists. splits. reflexivity.
+       - eexists. eexists. splits. reflexivity.
 Qed.
 
 (* Concrete Semantics *)
@@ -153,7 +150,8 @@ Fixpoint trace_of' (V0: Valuation) (t:CTrace) (s:Stmt) : CTrace :=
 Definition trace_of (V0:Valuation) (s:Stmt) : CTrace :=
   trace_of' V0 [] s.
 
-Definition has_trace__C (V0:Valuation) (s:Stmt) (t:CTrace) : Prop := t = trace_of V0 s.
+Definition has_trace__C (V0:Valuation) (s:Stmt) : Ensemble CTrace := Singleton _ (trace_of V0 s).
+
 
 Example branch_ex__C : has_trace__C (_ !-> 0) <{if X <= 1 {Y := X ; skip} {Y := 1}}> [CTAsgn Y 0].
 Proof. unfold has_trace__C, trace_of. simpl. unfold Aeval_t. simpl. reflexivity. Qed.
@@ -192,6 +190,32 @@ Definition pc_id := pc id_sub.
 
 Definition is_abstraction (V0:Valuation) (tc:CTrace) (ts:STrace) : Prop :=
   acc_val V0 tc = Comp V0 (acc_subst_id ts).
+
+Example completeness_branch_ex : is_abstraction (_ !-> 0) [CTAsgn Y 0] [STCond <{X <= 1}> ; STAsgn Y X]
+                       /\ Beval (_ !-> 0) (pc_id [STCond <{X <= 1}> ; STAsgn Y X]) = true.
+Proof. splits.
+  unfold is_abstraction, acc_subst_id, Comp. simpl. extensionality x.
+  unfold update. destruct (Y =? x); reflexivity.
+Qed.
+
+Example s_trace_ex := [STAsgn X 1 ; STAsgn Y 2; STAsgn X Y ; STAsgn Y X].
+Example completeness_par_ex : has_trace__S <{(X := 1 ; Y := 2) || (X := Y ; Y := X)}> s_trace_ex
+                              /\ is_abstraction (_ !-> 0) (trace_of (_ !-> 0) <{(X := 1 ; Y := 2) || (X := Y ; Y := X)}>) s_trace_ex
+                              /\ Beval (_ !-> 0) (pc_id s_trace_ex) = true.
+Proof.
+  splits.
+  - unfold has_trace__S, In. exists [STAsgn X 1; STAsgn Y 2]. exists [STAsgn X Y; STAsgn Y X]. splits.
+       + repeat constructor.
+       + eexists. eexists. splits. reflexivity.
+       + eexists. eexists. splits. reflexivity.
+  - unfold trace_of. simpl. unfold Aeval_t. simpl. rewrite 2 update_eq.
+    unfold is_abstraction. simpl.
+    unfold acc_subst_id, acc_subst, s_trace_ex. simpl. rewrite 2 update_eq.
+    extensionality x. unfold Comp, update.
+    (* lol *)
+    destruct (Y =? x); destruct (X =? X); destruct (Y =? Y); destruct (Y =? X); destruct (X =? Y); destruct (X =? x);
+      reflexivity.
+Qed.
 
 Lemma cond_idemp : forall b t s,
     acc_subst s (t :: STCond b) = acc_subst s t.
@@ -236,7 +260,71 @@ Proof.
     [|destruct a; simpl; rewrite IHt2]; reflexivity.
 Qed.
 
-Theorem soundness : forall s V0 , exists ts,
+Lemma interleave_degen : forall t1 t2, is_interleaving t1 t2 (t1 ++ t2).
+Proof.
+  intros. induction t2.
+  - constructor.
+  - simpl. constructor. assumption.
+Qed.
+
+Lemma par_all_left : forall s1 s2 t1 t2, has_trace__S s1 t1 -> has_trace__S s2 t2 -> has_trace__S <{s1 || s2}> (t1 ++ t2).
+Proof.
+  intros. exists t1. exists t2. splits.
+  - apply interleave_degen.
+  - assumption.
+  - assumption.
+Qed.
+
+Lemma is_abstraction_asgn : forall V0 t t' x e,
+    is_abstraction V0 t t' -> is_abstraction V0 (t::CTAsgn x (Aeval_t V0 t e)) (t'::STAsgn x e).
+Proof.
+  intros. unfold is_abstraction, acc_subst_id in *. simpl. unfold Aeval_t. rewrite H. simpl.
+  rewrite asgn_sound. reflexivity.
+Qed.
+
+Lemma is_abstraction_step : forall V0 t t' x, exists y,
+    is_abstraction V0 t t' -> is_abstraction V0 (t::x) (t'::y).
+Proof.
+  intros. dependent destruction x.
+  - exists (STAsgn x v). intro.
+    assert (v = Aeval_t V0 t v). { unfold Aeval_t. reflexivity. }
+    rewrite H0. apply is_abstraction_asgn. assumption.
+Qed.
+
+Lemma trace_acc_val : forall V0 t s, trace_of' V0 t s = trace_of (acc_val V0 t) s.
+Proof.
+  intros. induction t.
+  - simpl. unfold trace_of. reflexivity.
+  - destruct a; induction s.
+    + simpl. unfold trace_of. simpl. unfold Aeval_t. reflexivity.
+    + simpl in *. rewrite IHs1. unfold trace_of. subst; simpl.
+Admitted.
+
+Lemma pc_monotone : forall V0 t t', Beval V0 (pc_id (t ++ t')) = true ->
+                               Beval V0 (pc_id t) = true /\ Beval V0 (pc (acc_subst_id t) t') = true.
+Proof. intros. rewrite pc_app in H. apply andb_true_iff in H. assumption. Qed.
+
+Theorem soundness : forall V0 s t,
+    has_trace__S s t ->
+    Beval V0 (pc_id t) = true ->
+    exists t', has_trace__C V0 s t'
+          /\ is_abstraction V0 t' t.
+Proof.
+  intros. dependent induction s.
+  - exists [CTAsgn x (Aeval V0 e)]. splits.
+    + inversion H; subst. unfold is_abstraction, acc_subst_id. simpl.
+      rewrite asgn_sound. rewrite comp_id. reflexivity.
+  - inversion H. destruct H1 as [t' [Happ [Hs1 Hs2]]].
+    rewrite Happ in H0. apply pc_monotone in H0. destruct H0.
+    destruct (IHs1 x) as [t1 [t1Comp t1Abs]]; try assumption.
+    destruct (IHs2 t') as [t2 [t2Comp t2Abs]]; try assumption.
+    shelve.
+    exists (t1 ++ t2). splits.
+    + unfold has_trace__C in *. unfold trace_of in *. simpl.
+      rewrite trace_acc_val. rewrite <- t1Comp. rewrite <- t2Comp. simpl.
+      (* did I fuck up the definitions somehow? this all seems very off *)
+
+Theorem completeness : forall s V0 , exists ts,
     has_trace__S s ts /\ is_abstraction V0 (trace_of V0 s) ts /\ Beval V0 (pc_id ts) = true.
 Proof.
   intros.
@@ -244,20 +332,25 @@ Proof.
   dependent induction s.
   - (* x := e *)
     exists [STAsgn x e]. splits.
-    + apply htr_asgn.
-    + unfold is_abstraction. simpl. unfold acc_subst_id, acc_subst. simpl.
-      rewrite asgn_sound. rewrite comp_id. reflexivity.
+    + unfold trace_of. simpl. unfold is_abstraction, Aeval_t, acc_subst_id.
+      simpl. rewrite asgn_sound. rewrite comp_id. reflexivity.
   - (* s1 ; s2 *)
     destruct (IHs1 V0) as [ts1 [comp [IH1 IHpc1]]].
     destruct (IHs2 (acc_val V0 (trace_of V0 s1))) as [ts2 [comp2 [IH2 IHpc2]]].
     exists (ts1 ++ ts2). splits.
-    + apply htr_seq; assumption.
-    + unfold is_abstraction in *. rewrite trace_seq_app. rewrite acc_val_app.
-      unfold acc_subst_id. rewrite acc_subst_app.
-      rewrite IH1 in *. admit.
-    + rewrite pc_app. apply andb_true_iff. splits.
+    + eexists. eexists. splits; [apply comp | apply comp2].
+    + rewrite trace_seq_app. admit.
+    + rewrite pc_app. rewrite andb_true_iff. splits.
       * assumption.
-      * unfold is_abstraction in *. rewrite IH1 in IHpc2. rewrite comp_subB in IHpc2.
+      * unfold is_abstraction in IH1. rewrite IH1 in IHpc2.
+        rewrite comp_subB in IHpc2. unfold pc_id in IHpc2.
+
+  - (* s1 || s2 *)
+    destruct (IHs1 V0) as [ts1 [comp [IH1 IHpc1]]].
+    destruct (IHs2 (acc_val V0 (trace_of V0 s1))) as [ts2 [comp2 [IH2 IHpc2]]].
+    exists (ts1 ++ ts2). splits.
+    + apply par_all_left; assumption.
+    + unfold trace_of. simpl. unfold is_abstraction in *. rewrite acc_val_app.
 
       (* need some lemmas about multiple composition but I cannot formulate them separate from acc_*
        which is worrying *)
